Bipartite_Matching_LP.thy
@@ -1,0 +1,279 @@
+theory Bipartite_Matching_LP
+  imports
+    More_Graph
+    Jordan_Normal_Form.Matrix
+begin
+
+definition one_vec :: "nat \<Rightarrow> 'a :: one vec" ("1\<^sub>v") where
+  "1\<^sub>v n \<equiv> vec n (\<lambda>i. 1)"
+
+lemma one_carrier_vec[simp]: "1\<^sub>v n \<in> carrier_vec n"
+  unfolding one_vec_def carrier_vec_def by simp
+
+lemma index_one_vec[simp]: "i < n \<Longrightarrow> 1\<^sub>v n $ i = 1" "dim_vec (1\<^sub>v n) = n"
+  unfolding one_vec_def by simp_all
+
+lemma to_nat_on_from_nat_into_less:
+  assumes "finite A"
+  assumes "i < card A"
+  shows "to_nat_on A (from_nat_into A i) = i"
+  using assms
+  by (auto intro!: to_nat_on_from_nat_into dest!: to_nat_on_finite simp: bij_betw_def)
+
+lemma to_nat_on_less_card:
+  assumes "finite A"
+  assumes "a \<in> A"
+  shows "to_nat_on A a < card A"
+  using assms
+  by (auto dest: to_nat_on_finite bij_betwE)
+
+locale bipartite_matching_lp = 
+  fixes L :: "'a set" and R :: "'a set"
+  fixes G :: "'a graph"
+
+  assumes finite_L: "finite L" and finite_R: "finite R"
+  assumes bipartite_graph: "bipartite G L R"
+  assumes parts_minimal: "Vs G = L \<union> R"
+begin
+
+sublocale graph_abs G
+  using bipartite_graph finite_L finite_R
+  by (intro finite_parts_bipartite_graph_abs)
+
+lemmas finite_graph[intro,simp] = finite_E
+lemmas finite_vs[intro] = graph[THEN conjunct2]
+
+lemma parts_disjoint[intro,simp]: "L \<inter> R = {}"
+  using bipartite_graph
+  by (auto dest: bipartite_disjointD)
+
+lemma bipartite_FalseD[dest]:  "x \<in> L \<Longrightarrow> x \<in> R \<Longrightarrow> False"
+  using bipartite_graph
+  by (auto dest: bipartite_disjointD)
+
+definition "n \<equiv> card (Vs G)"
+definition "m \<equiv> card G"
+
+definition Vs_enum :: "'a \<Rightarrow> nat" where
+  "Vs_enum x \<equiv> if x \<in> L then to_nat_on L x else to_nat_on R x + card L"
+
+definition Vs_enum_inv :: "nat \<Rightarrow> 'a" where
+  "Vs_enum_inv i \<equiv> if i < card L then from_nat_into L i else from_nat_into R (i - card L)"
+
+abbreviation G_enum :: "'a set \<Rightarrow> nat" where
+  "G_enum \<equiv> to_nat_on G"
+
+definition incidence_matrix :: "real mat" where
+  "incidence_matrix \<equiv> mat n m (\<lambda>(i,j). of_bool (Vs_enum_inv i \<in> from_nat_into G j))"
+
+definition primal_sol :: "'a graph \<Rightarrow> real vec" where
+  "primal_sol M \<equiv> vec m (\<lambda>i. of_bool (from_nat_into G i \<in> M))"
+
+lemma dim_primal_sol[simp]: "dim_vec (primal_sol M) = m"
+  by (simp add: primal_sol_def)
+
+lemma n_sum: "n = card L + card R"
+  using parts_minimal finite_L finite_R
+  by (auto simp: card_Un_disjoint n_def)
+
+lemma geq_L_less_n_less_R: "card L \<le> i \<Longrightarrow> i < n \<Longrightarrow> i - card L < card R"
+  by (auto simp: n_sum)
+
+lemma geq_L_less_n_less_R': "\<not> i < card L \<Longrightarrow> i < n \<Longrightarrow> i - card L < card R"
+  by (auto intro: geq_L_less_n_less_R)
+
+lemma Vs_cases: 
+  assumes "x \<in> Vs G"
+  obtains "x \<in> L \<and> x \<notin> R" | "x \<in> R \<and> x \<notin> L"
+  using assms parts_minimal
+  by auto
+
+lemma i_cases:
+  assumes "i < n"
+  obtains "i < card L" | "card L \<le> i" "i < card L + card R"
+  using assms
+  by (auto simp: n_sum) linarith
+
+lemma
+  shows L_inv_enum[simp]: "l \<in> L \<Longrightarrow> from_nat_into L (to_nat_on L l) = l"
+    and L_enum_inv[simp]: "i < card L \<Longrightarrow> to_nat_on L (from_nat_into L i) = i"
+    and R_inv_enum[simp]: "r \<in> R \<Longrightarrow> from_nat_into R (to_nat_on R r) = r"
+    and R_enum_inv[simp]: "j < card R \<Longrightarrow> to_nat_on R (from_nat_into R j) = j"
+  using finite_L finite_R
+  by (auto simp: countable_finite intro: to_nat_on_from_nat_into_less)
+
+lemma
+  shows L_enum_less_card: "l \<in> L \<Longrightarrow> to_nat_on L l < card L"
+    and R_enum_less_card: "r \<in> R \<Longrightarrow> to_nat_on R r < card R"
+  using finite_L finite_R
+  by (auto intro: to_nat_on_less_card)
+
+lemma
+  shows L_enum_less_n: "l \<in> L \<Longrightarrow> to_nat_on L l < n"
+    and R_enum_less_n: "r \<in> R \<Longrightarrow> to_nat_on R r + card L < n"
+  by (auto simp: n_sum dest: L_enum_less_card R_enum_less_card)
+
+lemma
+  shows Vs_enum_L: "l \<in> L \<Longrightarrow> Vs_enum l = to_nat_on L l"
+    and Vs_enum_inv_from_nat_into_L: "i < card L \<Longrightarrow> Vs_enum_inv i = from_nat_into L i"
+  unfolding Vs_enum_def Vs_enum_inv_def
+  by auto
+
+lemma
+  shows Vs_enum_R: "r \<in> R \<Longrightarrow> Vs_enum r = to_nat_on R r + card L"
+    and "card L \<le> i \<Longrightarrow> Vs_enum_inv i = from_nat_into R (i - card L)"
+  unfolding Vs_enum_def Vs_enum_inv_def
+  by auto
+
+lemma Vs_enum_less_n: "x \<in> Vs G \<Longrightarrow> Vs_enum x < n"
+  by (auto elim!: Vs_cases simp: Vs_enum_L Vs_enum_R intro: L_enum_less_n R_enum_less_n)
+
+lemma 
+  shows Vs_enum_less_n_L: "i \<in> L \<Longrightarrow> Vs_enum i < n"
+    and Vs_enum_less_n_R: "j \<in> R \<Longrightarrow> Vs_enum j < n"
+  by (auto simp: parts_minimal intro: Vs_enum_less_n)
+
+lemma
+  shows Vs_inv_enum[simp]: "x \<in> Vs G \<Longrightarrow> Vs_enum_inv (Vs_enum x) = x"
+    and Vs_enum_inv[simp]: "i < n \<Longrightarrow> Vs_enum (Vs_enum_inv i) = i"
+  using finite_L finite_R
+  by (auto elim!: Vs_cases simp: Vs_enum_inv_def Vs_enum_def n_sum dest: L_enum_less_card intro!: from_nat_into)
+
+lemma
+  shows Vs_inv_enum_L[simp]: "i \<in> L \<Longrightarrow> Vs_enum_inv (Vs_enum i) = i"
+    and Vs_inv_enum_R[simp]: "j \<in> R \<Longrightarrow> Vs_enum_inv (Vs_enum j) = j"
+  by (simp_all add: parts_minimal)
+
+lemma Vs_enum_inv_leftE:
+  assumes "i < card L"
+  obtains j where "j \<in> L" "Vs_enum_inv i = j"
+  using assms
+  by (metis Vs_enum_inv_def card.empty from_nat_into not_less_zero)
+
+lemma Vs_enum_inv_rightE:
+  assumes "i < n"
+  assumes "\<not> i < card L"
+  obtains j where "j \<in> R" "Vs_enum_inv i = j"
+  using assms
+  by (metis Vs_enum_inv_def add.right_neutral card.empty from_nat_into n_sum)
+
+lemma G_not_empty_if:
+  assumes "i < m"
+  shows "G \<noteq> {}"
+  using assms
+  unfolding m_def
+  by fastforce
+
+lemma from_nat_into_G_E_aux:
+  assumes "i < m"
+  obtains e where "e \<in> G" "from_nat_into G i = e"
+  using assms
+  by (metis G_not_empty_if from_nat_into)
+
+lemma from_nat_into_G_E:
+  assumes "i < m"
+  obtains l r where "{l,r} \<in> G" "from_nat_into G i = {l,r}" "l \<in> L" "r \<in> R"
+  using assms bipartite_graph
+  by (metis bipartite_edgeE from_nat_into_G_E_aux)
+
+lemma Vs_enum_neqI: "v \<in> Vs G \<Longrightarrow> v' \<in> Vs G \<Longrightarrow> v \<noteq> v' \<Longrightarrow> Vs_enum v \<noteq> Vs_enum v'"
+  by (metis Vs_inv_enum)
+
+lemma G_enum_neqI: "e \<in> G \<Longrightarrow> e' \<in> G \<Longrightarrow> e \<noteq> e' \<Longrightarrow> G_enum e \<noteq> G_enum e'"
+  by (simp add: countable_finite)
+
+lemma primal_dot_One_card: "M \<subseteq> G \<Longrightarrow> primal_sol M \<bullet> (1\<^sub>v m) = card M"
+  by (auto simp: scalar_prod_def m_def primal_sol_def countable_finite in_mono
+           intro!: bij_betw_same_card[where f = "from_nat_into G"] bij_betwI[where g = G_enum] 
+                   to_nat_on_less_card to_nat_on_from_nat_into_less)
+
+lemma matching_feasible:
+  assumes "matching M"
+  shows "incidence_matrix *\<^sub>v primal_sol M \<le> 1\<^sub>v n"
+  unfolding incidence_matrix_def primal_sol_def 
+  apply (auto simp: mult_mat_vec_def scalar_prod_def less_eq_vec_def)
+proof (rule ccontr, simp add: not_le)
+  fix i
+  assume "i < n"
+  let ?indices = "{0..<m} \<inter> {e. from_nat_into G e \<in> M} \<inter> {e. local.Vs_enum_inv i \<in> from_nat_into G e}"
+  assume "1 < real (card ?indices)"
+
+  then have gt_1: "1 < card ?indices"
+    by simp
+
+  then obtain ei1 where ei1: "ei1 \<in> ?indices"
+    by (metis card_eq_0_iff ex_in_conv not_less0)
+
+  with gt_1 have "0 < card (?indices - {ei1})"
+    by auto
+
+  then obtain ei2 where ei2: "ei2 \<in> ?indices" "ei1 \<noteq> ei2"
+    by (metis Diff_eq_empty_iff card_0_eq card_ge_0_finite insertCI not_gr_zero subsetI)
+
+  with ei1 have "from_nat_into G ei1 \<in> M" "from_nat_into G ei2 \<in> M" 
+    "Vs_enum_inv i \<in> from_nat_into G ei1" "Vs_enum_inv i \<in> from_nat_into G ei2"
+    by auto
+
+  with \<open>matching M\<close> have "from_nat_into G ei1 = from_nat_into G ei2"
+    by (auto dest: matching_unique_match)
+
+  with \<open>ei1 \<noteq> ei2\<close> show False  
+    by (metis IntD1 atLeastLessThan_iff ei1 ei2(1)finite_E m_def to_nat_on_from_nat_into_less)
+qed
+
+lemma feasible_matching:
+  assumes "M \<subseteq> G"
+  assumes "incidence_matrix *\<^sub>v primal_sol M \<le> 1\<^sub>v n"
+  shows "matching M"
+  using assms
+  unfolding incidence_matrix_def primal_sol_def mult_mat_vec_def scalar_prod_def less_eq_vec_def
+  apply auto
+proof (rule ccontr)
+  assume "M \<subseteq> G"
+  let ?indices = "\<lambda>i. {0..<m} \<inter> {i. from_nat_into G i \<in> M} \<inter> {x. Vs_enum_inv i \<in> from_nat_into G x}"
+  assume at_most_One: "\<forall>i<n. real (card (?indices i)) \<le> 1"
+  assume "\<not>matching M"
+
+  then obtain e1 e2 where "e1 \<in> M" "e2 \<in> M" "e1 \<noteq> e2" "e1 \<inter> e2 \<noteq> {}"
+    unfolding matching_def
+    by blast
+
+  then obtain v where "v \<in> e1" "v \<in> e2"
+    by blast
+
+  with \<open>e1 \<in> M\<close> have v_le_n: "Vs_enum v < n"
+    by (metis L_enum_less_n R_enum_less_n Vs_cases Vs_enum_def assms(1) subset_eq vs_member_intro)
+
+  have e1_in_indices: "G_enum e1 \<in> ?indices (Vs_enum v)"
+    by (smt (verit) IntI Vs_inv_enum \<open>e1 \<in> M\<close> \<open>v \<in> e1\<close> assms(1) atLeastLessThan_iff countable_finite from_nat_into_to_nat_on finite_E in_mono m_def mem_Collect_eq to_nat_on_less_card vs_member_intro zero_le)
+
+  have e2_in_indices: "G_enum e2 \<in> ?indices (Vs_enum v)"
+    by (smt (verit) IntI Vs_inv_enum \<open>e2 \<in> M\<close> \<open>v \<in> e2\<close> assms(1) atLeastLessThan_iff countable_finite from_nat_into_to_nat_on finite_E in_mono m_def mem_Collect_eq to_nat_on_less_card vs_member_intro zero_le)
+
+  have "G_enum e1 \<noteq> G_enum e2"
+    using G_enum_neqI \<open>e1 \<in> M\<close> \<open>e1 \<noteq> e2\<close> \<open>e2 \<in> M\<close> assms(1) by blast
+
+  then have "0 < card (?indices (Vs_enum v) - {G_enum e2})"
+    by (metis Diff_cancel Diff_iff card_gt_0_iff e1_in_indices finite_Diff finite_Int finite_atLeastLessThan insertE)
+
+  then have "1 < card (?indices (Vs_enum v))"
+    by (metis Diff_empty card_Diff_insert e2_in_indices empty_iff zero_less_diff)
+
+  also from at_most_One v_le_n have "\<dots> \<le> 1"
+    by auto
+
+  finally have "1 < 1" ..
+
+  then show False
+    by fast
+qed
+
+lemma matching_iff_feasible:
+  assumes "M \<subseteq> G"
+  shows "matching M \<longleftrightarrow> incidence_matrix *\<^sub>v primal_sol M \<le> 1\<^sub>v n"
+  using assms
+  by (auto intro: feasible_matching matching_feasible)
+
+end
+
+end
